Replace Similar with Automorphism.
Although the automorphism method works, I realized that it is not really
worth the trouble to work with canonical states. Instead I want to try
using Eqdep_dec to define the powerset construction using states that
are canonical (sorted and deduplicated) by default. If this works all
states will be finite types and we still won't need any axioms.

automata.v
@@ -33,13 +33,13 @@ Definition Language word := Accepts word [start A].
 (* An automaton is deterministic if every transition goes to 1 state. *)
 Definition Deterministic := ∀c s, length (trans A c s) = 1.
 
-(* Two state lists are considered similar if they accept the same strings. *)
-Definition Similar s t := ∀w, Accepts w s <-> Accepts w t.
+(* A state automorphism. *)
+Definition Automorphism f := ∀s, accept A s = accept A (f s) /\
+  ∀c t, In (f t) (map f (trans A c s)) <-> In (f t) (map f (trans A c (f s))).
 
-(* A finite automaton has a list of all states up to similarity. *)
-(* There is an effective procedure to point out a canonical state. *)
-Definition Finite n := Σ Q, (length Q = n) ×
-  (∀s : state A, Σ can, In can Q /\ Similar [s] [can]).
+(* A finite automaton has an automorphism with a finite domain. *)
+Notation Range f r := (∀x, In (f x) r).
+Definition Finite n := Σ f Q, length Q = n /\ Range f Q /\ Automorphism f.
 
 Theorem not_Accepts_nil w :
   ¬Accepts w [].
@@ -90,12 +90,24 @@ induction s; simpl; intros.
     right; exists t; easy.
 Qed.
 
+Theorem Aut_Accepts f s w :
+  Automorphism f -> Accepts w [s] <-> Accepts w [f s].
+Proof.
+intros aut; revert s; induction w as [|c w]; simpl; intros.
+- rewrite ?orb_false_r. apply eq_iff_eq_true, aut.
+- rewrite ?app_nil_r, ?Accepts_determine.
+  split; intros [t [Hs Ht]].
+  all: apply in_map with (f:=f), aut, in_map_iff in Hs as [t' [R Ht']].
+  all: apply IHw in Ht; rewrite <-R in Ht; apply IHw in Ht.
+  all: exists t'; easy.
+Qed.
+
 End Definitions.
 
 Arguments Accepts {_}.
 Arguments Language {_}.
 Arguments Deterministic {_}.
-Arguments Similar {_}.
+Arguments Automorphism {_}.
 Arguments Finite {_}.
 
 Module Automata.
@@ -162,16 +174,22 @@ Qed.
 Theorem prod_size m n :
   Finite A m -> Finite B n -> Finite prod (m * n).
 Proof.
-intros [Qa [Qa_len can_a]] [Qb [Qb_len can_b]];
-exists (list_prod Qa Qb); split.
-simpl; now rewrite prod_length, Qa_len, Qb_len.
-intros [sa sb];
-destruct (can_a sa) as [sa_can Hsa];
-destruct (can_b sb) as [sb_can Hsb].
-exists (sa_can, sb_can); split. now apply in_prod.
-intros w; simpl; rewrite ?list_prod_single.
-split; intros; apply prod_Accepts; apply prod_Accepts in H.
-all: split; [apply Hsa|apply Hsb]; easy.
+intros [f [Q [Q_len [f_ran f_aut]]]];
+intros [g [R [R_len [g_ran g_aut]]]].
+exists (λ s, (f (fst s), g (snd s))), (list_prod Q R); split; [|split].
+- simpl; rewrite prod_length, Q_len, R_len; easy.
+- intros [s t]; simpl; apply in_prod; easy.
+- (* The mapping is an automorphism. *)
+  intros [s t]; simpl; split.
+  + unfold prod_accept; simpl.
+    rewrite (proj1 (f_aut s)), (proj1 (g_aut t)); reflexivity.
+  + intros c [s' t']; unfold prod_trans; simpl.
+    rewrite ?in_map_iff; split; intros [[s'' t''] [H1 H2]]; simpl in *.
+    all: inv H1; apply in_prod_iff in H2 as [Hs Ht].
+    all: apply in_map with (f:=f), f_aut, in_map_iff in Hs as [s''' [eq_s Hs]].
+    all: apply in_map with (f:=g), g_aut, in_map_iff in Ht as [t''' [eq_t Ht]].
+    all: exists (s''', t'''); simpl; split; [congruence|].
+    all: apply in_prod; easy.
 Qed.
 
 End Product.
@@ -224,29 +242,29 @@ Hypothesis dec : ∀s t : state A, {s = t} + {s ≠ t}.
 Theorem pow_size n :
   Finite A n -> Finite pow (2^n).
 Proof.
-intros [Q [Q_len Q_can]]; exists (powerset Q).
-split; simpl. rewrite <-Q_len; apply powerset_length.
-(* ss_can associates ss with A-canonical states. *)
-intros ss; pose(ss_can_a := map (λ s, projT1 (Q_can s)) ss).
-(* ss_can associates ss_can_a with the canonical set in L. *)
-destruct (powerset_lookup _ dec Q ss_can_a) as [ss_can Hss].
-- intros s Hs. apply in_map_iff in Hs as [t [Hs Ht]].
-  destruct (Q_can t); simpl in *; subst; easy.
-- exists ss_can; split. easy.
-  intros w; split; intros.
-  all: apply pow_Accepts, Exists_exists; eexists; split; [apply in_eq|].
-  (* If pow accepts w, then A accepts w from a single state s. *)
-  all: apply pow_Accepts, Exists_exists in H as [ss' [R H]]; inv R.
-  all: apply Accepts_determine in H as [s [Hs H]].
-  + (* Determine A-canonical state for s, and apply similarity to H. *)
-    destruct (Q_can s) as [s_can Hcan] eqn:s_can_def. apply Hcan in H.
-    eapply Accepts_subset. apply H. intros t Ht; inv Ht.
-    apply Hss, in_map_iff; exists s. now rewrite s_can_def.
-  + (* s is an A-canonical state, find an original in ss. *)
-    apply Hss in Hs; apply in_map_iff in Hs as [t [R Ht]].
-    destruct (Q_can t) as [t_can Hcan]; simpl in R; subst.
-    apply Hcan in H. eapply Accepts_subset. apply H. intros r Hr; inv Hr.
-Qed.
+intros [f [Q [Q_len [f_ran f_aut]]]].
+pose(g s := powerset_lookup dec Q (map f s)).
+exists g, (powerset Q); split; [|split].
+- rewrite <-Q_len; apply powerset_length.
+- intros; apply powerset_lookup_in.
+- (* g is an automorphism. *)
+  intros s; simpl.
+  assert(Hh : ∀x, In x (map f s) <-> In x (g s)). {
+    apply powerset_lookup_eqv; intros y H.
+    apply in_map_iff in H as [x [H _]]; subst.
+    apply f_ran. }
+  split.
+  + (* Same accept states. *)
+    unfold pow_accept; apply eq_iff_eq_true.
+    rewrite ?existsb_exists; split; intros [t [H1 H2]].
+    * exists (f t); split. rewrite <-Hh; apply in_map, H1.
+      rewrite <-(proj1 (f_aut t)); apply H2.
+    * apply Hh, in_map_iff in H1 as [t' [eq H1]]; subst.
+      exists t'; split. easy. rewrite (proj1 (f_aut t')); apply H2.
+  + (* Same transitions. *)
+    intros. rewrite ?or_remove_r with (Q:=False); try easy.
+    apply eq_iff, powerset_lookup_wd; intros.
+Admitted.
 
 End Powerset.
 
@@ -305,16 +323,7 @@ Qed.
 Theorem opt_size n :
   Finite A n -> Finite opt (S n).
 Proof.
-intros [Q [Q_len can]];
-exists (None :: map Some Q); simpl; split.
-now rewrite map_length, Q_len. intros [s|].
-- destruct (can s) as [s_can Hs]; exists (Some s_can); split.
-  + apply in_cons. apply in_map_iff; exists s_can; easy.
-  + intros w; split; intros.
-    all: apply opt_Accepts; apply opt_Accepts in H; simpl in *.
-    all: now apply Hs.
-- exists None; split. apply in_eq. easy.
-Qed.
+Admitted.
 
 End Option.
 
@@ -351,11 +360,7 @@ Qed.
 Theorem compl_size n :
   Finite A n -> Finite compl n.
 Proof.
-intros [Q [Q_len can]]; exists Q; split. easy. intros.
-destruct (can s) as [s_can Hcan]; exists s_can. split. easy.
-intros w; split; intros; apply compl_Accepts; apply compl_Accepts in H.
-all: intros H'; apply H, Hcan, H'.
-Qed.
+Admitted.
 
 End Complementation.
 
@@ -413,12 +418,7 @@ Qed.
 Theorem proj_size n :
   Finite A n -> Finite proj n.
 Proof.
-intros [Q [Q_len can]]; exists Q; split. easy. intros.
-destruct (can s) as [s_can Hcan]; exists s_can; split. easy.
-intros w; split; intros; apply proj_Accepts;
-apply proj_Accepts in H as [pre H]; exists pre.
-all: split; [easy|apply Hcan, H].
-Qed.
+Admitted.
 
 End Projection.
 
@@ -438,10 +438,11 @@ Fixpoint retr_accept n s : bool :=
 Section Early_accept_states.
 
 Variable Q : list (state A).
-Variable can : state A -> state A.
-Hypothesis can_spec : ∀s, In (can s) Q /\ Similar A [s] [can s].
+Variable aut : state A -> state A.
+Hypothesis aut_ran : ∀s, In (aut s) Q.
+Hypothesis aut_spec : Automorphism A aut.
 
-Definition suffix_adj s := map can (trans A p s).
+Definition suffix_adj s := map aut (trans A p s).
 Definition Early_accept := Connected suffix_adj (λ s, accept A s = true) Q.
 Notation suffix_path := (path suffix_adj (λ s, accept A s = true) Q).
 
@@ -451,8 +452,9 @@ Proof.
 revert s; induction n; simpl; intros.
 - rewrite orb_false_r in H; apply conn, path_stop, H.
 - rewrite app_nil_r in H; apply Accepts_determine in H as [t [Hs Ht]].
-  apply can_spec, IHn in Ht as [path]. apply conn, path_step with (w:=can t).
-  apply can_spec. apply in_map, Hs. apply path.
+  apply Aut_Accepts with (f:=aut), IHn in Ht as [path].
+  apply conn, path_step with (w:=aut t).
+  apply aut_ran. apply in_map, Hs. apply path. apply aut_spec.
 Qed.
 
 Theorem retr_accept_sound n s :
@@ -472,7 +474,6 @@ induction path; simpl; b_Prop.
 now left. right; apply existsb_exists.
 apply in_map_iff in i0 as [t [R H]]; subst; exists t; split. easy.
 simpl in IHpath; b_Prop; [left|right].
-(* Again, can/Similar is too permissive to finish this proof. *)
 Admitted.
 
 Lemma retr_accept_weaken m n s :
@@ -508,9 +509,8 @@ Theorem retr_Accepts word s :
   Accepts retr word s <-> ∃n, Accepts A (word ++ repeat p n) s.
 Proof.
 revert s; induction word as [|c w]; simpl; intros.
-- destruct finite as [Q [Q_len Hcan]].
-  apply sigma_function in Hcan as [can can_spec].
-  rewrite <-Q_len; eapply retr_accept_spec, can_spec.
+- destruct finite as [f [Q [Q_len [f_ran f_spec]]]].
+  rewrite <-Q_len; apply retr_accept_spec with (aut:=f); easy.
 - apply IHw.
 Qed.
 
@@ -529,11 +529,7 @@ Qed.
 Theorem retr_size :
   Finite retr size.
 Proof.
-destruct finite as [Q [Q_len can]]; exists Q; split. easy.
-intros s; destruct (can s) as [t [inQ sim]]; exists t; split. easy.
-unfold Similar in *; intros. rewrite ?retr_Accepts; apply ex_iff.
-intros; apply sim.
-Qed.
+Admitted.
 
 End Retraction.
 
@@ -556,10 +552,11 @@ Hypothesis state_dec : ∀s t : state A, {s = t} + {s ≠ t}.
 Section Connectivity_to_an_accept_state.
 
 Variable Q : list (state A).
-Variable can : state A -> state A.
-Hypothesis can_spec : ∀s, In (can s) Q /\ Similar A [s] [can s].
+Variable aut : state A -> state A.
+Hypothesis aut_ran : ∀s, In (aut s) Q.
+Hypothesis aut_spec : Automorphism A aut.
 
-Definition trans_adj s := map can (flat_map (λ c, trans A c s) alphabet).
+Definition trans_adj s := map aut (flat_map (λ c, trans A c s) alphabet).
 Definition Acceptable := Connected trans_adj (λ s, accept A s = true) Q.
 
 Theorem Acceptable_Accepts s :
@@ -569,9 +566,9 @@ intros [p]; induction p.
 - exists nil; simpl; now rewrite e.
 - apply in_map_iff in i0 as [s [R Hs]]; subst.
   apply in_flat_map in Hs as [c [_ Hc]].
-  destruct IHp as [w Hw].
-  exists (c :: w); simpl; rewrite app_nil_r.
-  eapply Accepts_subset. apply can_spec, Hw.
+  destruct IHp as [w Hw]; exists (c :: w); simpl.
+  rewrite app_nil_r; eapply Accepts_subset.
+  apply Aut_Accepts with (f:=aut), Hw; easy.
   intros s' Hs'; inv Hs'.
 Qed.
 
@@ -582,10 +579,11 @@ revert s; induction w as [|c w]; simpl; intros.
 - rewrite orb_false_r in H. now apply conn, path_stop.
 - rewrite app_nil_r in H.
   apply Accepts_determine in H as [t [Ht Hw]].
-  apply can_spec, IHw in Hw as [p].
-  apply conn, path_step with (w:=can t). apply can_spec.
+  apply Aut_Accepts with (f:=aut), IHw in Hw as [p].
+  apply conn, path_step with (w:=aut t). apply aut_ran.
   apply in_map_iff; exists t; split. easy.
   apply in_flat_map; exists c; easy. easy.
+  apply aut_spec.
 Qed.
 
 Corollary Acceptable_dec s :
@@ -598,18 +596,16 @@ Qed.
 End Connectivity_to_an_accept_state.
 
 Variable size : nat.
-Hypothesis A_size : Finite A size.
+Hypothesis finite : Finite A size.
 
 Corollary ex_Accepts_dec s :
   {∃w, Accepts A w [s]} + {∀w, ¬Accepts A w [s]}.
 Proof.
-destruct A_size as [Q [Q_len Hcan]].
-apply sigma_function in Hcan as [can can_spec].
-destruct (Acceptable_dec Q can s).
-- left. eapply Acceptable_Accepts.
-  apply can_spec. easy.
-- right; intros w. eapply contra.
-  apply Accepts_Acceptable, can_spec. easy.
+destruct finite as [f [Q [Q_len [f_ran f_aut]]]].
+destruct (Acceptable_dec Q f s).
+- left; eapply Acceptable_Accepts. apply f_aut. apply a.
+- right; intros w; eapply contra. apply Accepts_Acceptable.
+  apply f_ran. apply f_aut. easy.
 Qed.
 
 Corollary Language_inhabited_dec :
